Clean/Circuit/Extensions.lean
@@ -39,10 +39,9 @@ theorem witnessAny_localWitnesses (n : ℕ) (env : Environment F) :
     ProvableType.toElements_fromElements]
 
 @[circuit_norm]
-theorem witnessAny_interactionsWithChannel {n : ℕ} {channel : RawChannel F} {env : Environment F} :
-    (witnessAny α |>.operations n).interactionsWithChannel channel env = [] := by
-  simp only [circuit_norm, getOffset, witnessAny, valueFromOffset,
-    ProvableType.toElements_fromElements]
+theorem witnessAny_interactionsWith {n : ℕ} {channel : RawChannel F} :
+    (witnessAny α |>.operations n).interactionsWith channel = [] := by
+  simp [circuit_norm, witnessAny, valueFromOffset, ProvableType.toElements_fromElements]
 
 @[circuit_norm]
 theorem witnessAny_output {n : ℕ} :
