Clean/Circuit/Foundations.lean
@@ -21,7 +21,7 @@ open Circuit (ConstraintsHold)
 theorem FormalCircuit.original_soundness (circuit : FormalCircuit F β α) :
     ∀ (offset : ℕ) env (b_var : Var β F) (b : β F), eval env b_var = b → circuit.Assumptions b →
     -- if the constraints hold (original definition)
-    ConstraintsHold env (circuit.main b_var |>.operations offset) →
+    Operations.ConstraintsHold env (circuit.main b_var |>.operations offset) →
     -- the spec holds
     let a := eval env (circuit.output b_var offset)
     circuit.Spec b a := by
@@ -40,7 +40,7 @@ theorem FormalCircuit.original_completeness (circuit : FormalCircuit F β α) :
     -- if the environment uses default witness generators (original definition)
     env.UsesLocalWitnesses offset (circuit.main b_var |>.operations offset) →
     -- the constraints hold (original definition)
-    ConstraintsHold env (circuit.main b_var |>.operations offset) := by
+    Operations.ConstraintsHold env (circuit.main b_var |>.operations offset) := by
 
   intro offset env b_var b h_input h_assumptions h_env
   have h_env' := Environment.can_replace_usesLocalWitnessesCompleteness (circuit.subcircuitsConsistent ..) h_env
@@ -57,7 +57,7 @@ theorem FormalCircuit.original_completeness (circuit : FormalCircuit F β α) :
 theorem FormalAssertion.original_soundness (circuit : FormalAssertion F β) :
     ∀ (offset : ℕ) env (b_var : Var β F) (b : β F), eval env b_var = b → circuit.Assumptions b →
     -- if the constraints hold (original definition)
-    ConstraintsHold env (circuit.main b_var |>.operations offset) →
+    Operations.ConstraintsHold env (circuit.main b_var |>.operations offset) →
     -- the spec holds
     circuit.Spec b := by
 
@@ -75,7 +75,7 @@ theorem FormalAssertion.original_completeness (circuit : FormalAssertion F β) :
     -- if the environment uses default witness generators (original definition)
     env.UsesLocalWitnesses offset (circuit.main b_var |>.operations offset) →
     -- the spec implies that the constraints hold (original definition)
-    circuit.Spec b → ConstraintsHold env (circuit.main b_var |>.operations offset) := by
+    circuit.Spec b → Operations.ConstraintsHold env (circuit.main b_var |>.operations offset) := by
 
   intro offset env b_var b h_input h_assumptions h_env h_spec
   have h_env' := Environment.can_replace_usesLocalWitnessesCompleteness (circuit.subcircuitsConsistent ..) h_env
@@ -91,31 +91,18 @@ theorem FormalAssertion.original_completeness (circuit : FormalAssertion F β) :
 -/
 theorem FormalCircuitWithInteractions.original_full_soundness
     (circuit : FormalCircuitWithInteractions F β α) :
-    ∀ (offset : ℕ) env (b_var : Var β F) (b : β F), eval env b_var = b →
-    ConstraintsHold env (circuit.main b_var |>.operations offset) →
-    Operations.FullGuarantees env (circuit.main b_var |>.operations offset) →
-    let a := eval env (circuit.output b_var offset)
-    circuit.Spec b a env ∧
-      Operations.FullRequirements env (circuit.main b_var |>.operations offset) := by
-  intro offset env b_var b h_input h_constraints h_full_guarantees
-  have h_guarantees_flat :
-      FlatOperation.Guarantees env ((circuit.main b_var |>.operations offset).toFlat) := by
-    exact (FlatOperation.forAll_toFlat_iff
-      (condition := { interact i := i.assumeGuarantees → i.Guarantees env })
-      (ops := (circuit.main b_var |>.operations offset))).2 h_full_guarantees
-  have h_soundness_input :
-      ConstraintsHoldWithInteractions.Soundness env (circuit.main b_var |>.operations offset) :=
-    Circuit.can_replace_soundness h_constraints h_guarantees_flat
-  have h_soundness := circuit.soundness offset env b_var b h_input h_soundness_input
-  have h_req_flat :
-      FlatOperation.Requirements env ((circuit.main b_var |>.operations offset).toFlat) :=
-    Circuit.requirements_toFlat_of_soundness h_constraints h_guarantees_flat h_soundness.2
-  have h_full_req :
-      Operations.FullRequirements env (circuit.main b_var |>.operations offset) := by
-    exact (FlatOperation.forAll_toFlat_iff
-      (condition := { interact i := i.Requirements env })
-      (ops := (circuit.main b_var |>.operations offset))).1 h_req_flat
-  exact ⟨ h_soundness.1, h_full_req ⟩
+    ∀ (offset : ℕ) env (input_var : Var β F),
+    let ops := circuit.main input_var |>.operations offset;
+    let input := eval env input_var;
+    let output := eval env (circuit.output input_var offset);
+    ops.ConstraintsHold env → ops.FullGuarantees env →
+    circuit.Spec input output env ∧ ops.FullRequirements env := by
+  intro offset env input_var ops input output h_constraints h_full_guarantees
+  have h_soundness_input : ConstraintsHoldWithInteractions.Soundness env ops :=
+    Circuit.can_replace_soundness h_constraints h_full_guarantees
+  have ⟨ h_spec, h_requirements ⟩ := circuit.soundness offset env input_var input rfl h_soundness_input
+  use h_spec
+  apply Circuit.requirements_toFlat_of_soundness h_constraints h_full_guarantees h_requirements
 
 /--
   Foundational completeness theorem for circuits with interactions:
@@ -123,20 +110,13 @@ theorem FormalCircuitWithInteractions.original_full_soundness
 -/
 theorem FormalCircuitWithInteractions.original_full_completeness
     (circuit : FormalCircuitWithInteractions F β α) :
-    ∀ (offset : ℕ) env (b_var : Var β F) (b : β F), eval env b_var = b →
-    env.UsesLocalWitnesses offset (circuit.main b_var |>.operations offset) →
-    circuit.Assumptions b env →
-    ConstraintsHold env (circuit.main b_var |>.operations offset) ∧
-      Operations.FullGuarantees env (circuit.main b_var |>.operations offset) := by
-  intro offset env b_var b h_input h_env h_assumptions
-  have h_env' := Environment.can_replace_usesLocalWitnessesCompleteness (circuit.subcircuitsConsistent ..) h_env
-  have h_compl :=
-    circuit.completeness offset env b_var h_env' b h_input h_assumptions
-  have h_pair :=
-    Circuit.can_replace_completeness_and_guarantees (circuit.subcircuitsConsistent ..) h_env h_compl
-  have h_full_guarantees :
-      Operations.FullGuarantees env (circuit.main b_var |>.operations offset) := by
-    exact (FlatOperation.forAll_toFlat_iff
-      (condition := { interact i := i.assumeGuarantees → i.Guarantees env })
-      (ops := (circuit.main b_var |>.operations offset))).1 h_pair.2
-  exact ⟨ h_pair.1, h_full_guarantees ⟩
+    ∀ (offset : ℕ) env (input_var : Var β F),
+    let ops := circuit.main input_var |>.operations offset;
+    let input := eval env input_var;
+    env.UsesLocalWitnesses offset ops → circuit.Assumptions input env →
+    ops.ConstraintsHold env ∧ ops.FullGuarantees env := by
+  intro offset env input_var ops input h_env h_assumptions
+  have h_consistent := circuit.subcircuitsConsistent input_var offset
+  apply Circuit.can_replace_completeness_and_guarantees h_consistent h_env
+  have h_env' := env.can_replace_usesLocalWitnessesCompleteness h_consistent h_env
+  exact circuit.completeness offset env input_var h_env' input rfl h_assumptions
